code/ecdsa/Hacl.Impl.P256.Compression.fsti
@@ -28,7 +28,7 @@ inline_for_extraction
 val decompressionNotCompressedForm: #c: curve -> b: notCompressedForm c -> result: lbuffer uint8 (getCoordinateLenU c *! 2ul) -> Stack bool 
   (requires fun h -> live h b /\ live h result /\ disjoint b result)
   (ensures fun h0 r h1 -> modifies (loc result) h0 h1 /\ (
-    let len = v (getCoordinateLenU c) in 
+    let len = getCoordinateLen c in 
     
     let id = Lib.Sequence.index (as_seq h0 b) 0 in 
     let x = Lib.Sequence.sub (as_seq h0 b) 1 len in 
@@ -43,58 +43,60 @@ val decompressionNotCompressedForm: #c: curve -> b: notCompressedForm c -> resul
 
 
 inline_for_extraction
-val decompressionCompressedForm: #c: curve -> b: compressedForm -> result: lbuffer uint8 (size 64) -> Stack bool 
+val decompressionCompressedForm: #c: curve -> b: compressedForm c 
+  -> result: lbuffer uint8 (getCoordinateLenU c *! 2ul) -> Stack bool 
   (requires fun h -> live h b /\ live h result /\ disjoint b result)
-  (ensures fun h0 r h1 -> 
-    (
-      let id = Lib.Sequence.index (as_seq h0 b) 0 in 
-      let xSequence = Lib.Sequence.sub (as_seq h0 b) 1 32 in 
-      let x =  Lib.ByteSequence.nat_from_bytes_be xSequence in 
-      if uint_v id = 2 || uint_v id = 3 then
-	if x < prime256 then 
-	  r == true /\ 
-	  (
-	    let y = 
-              let sq = sq_root_spec  #c #DH (((x * x * x + aCoordinate #P256 * x + bCoordinate #P256) % prime256)) in 
-              if (uint_v id) % 2 = (sq % 2) then 
-		sq
-              else
-	         (0 - sq) % prime256 
-	    in 
-	    as_seq h1 (gsub result (size 0) (size 32)) == xSequence /\
-	    as_seq h1 (gsub result (size 32) (size 32)) == Lib.ByteSequence.nat_to_bytes_be 32 y)
-	else 
-	  r == false
+  (ensures fun h0 r h1 -> modifies (loc result) h0 h1 /\ (
+    let len = getCoordinateLen c in 
+    let prime = getPrime c in 
+    
+    let id = Lib.Sequence.index (as_seq h0 b) 0 in 
+    let xSequence = Lib.Sequence.sub (as_seq h0 b) 1 len in 
+    let x =  Lib.ByteSequence.nat_from_bytes_be xSequence in 
+
+    if uint_v id = 2 || uint_v id = 3 then
+      if x < prime then 
+	r == true /\ (
+	let y = 
+	  let sq = sq_root_spec #c #DH (((x * x * x + aCoordinate #c * x + bCoordinate #c) % prime)) in 
+	  if (uint_v id) % 2 = sq % 2 then 
+	    sq
+	  else
+	    (0 - sq) % prime in 
+	as_seq h1 (gsub result (size 0) (getCoordinateLenU c)) == xSequence /\
+	as_seq h1 (gsub result (getCoordinateLenU c) (getCoordinateLenU c)) == Lib.ByteSequence.nat_to_bytes_be len y)
       else 
-	r == false) /\
-  modifies (loc result) h0 h1)
+	r == false
+    else 
+      r == false))
+ 
 
 inline_for_extraction
-val compressionNotCompressedForm: #c: curve -> b: lbuffer uint8 (size 64) -> result: notCompressedForm -> 
-  Stack unit 
-    (requires fun h -> live h b /\ live h result /\ disjoint b result)
-    (ensures fun h0 _ h1 -> modifies (loc result) h0 h1 /\
-      (
-	let id = Lib.Sequence.index (as_seq h1 result) 0 in 
-	let x = Lib.Sequence.sub (as_seq h0 b) 0 32 in 
-	  let xResult = Lib.Sequence.sub (as_seq h1 result) 1 32 in 
-	let y = Lib.Sequence.sub (as_seq h0 b) 32 32 in 
-	  let yResult = Lib.Sequence.sub (as_seq h1 result) 33 32 in 
-	uint_v id == 4 /\ xResult == x /\ yResult == y 	
-      )
-    )
+val compressionNotCompressedForm: #c: curve -> b: lbuffer uint8 (getCoordinateLenU c *! 2ul) 
+  -> result: notCompressedForm c -> Stack unit 
+  (requires fun h -> live h b /\ live h result /\ disjoint b result)
+  (ensures fun h0 _ h1 -> modifies (loc result) h0 h1 /\ (
+    let len = getCoordinateLen c in
+    
+    let id = Lib.Sequence.index (as_seq h1 result) 0 in 
+    let x = Lib.Sequence.sub (as_seq h0 b) 0 len in 
+    let y = Lib.Sequence.sub (as_seq h0 b) len len in 
+    
+    let xResult = Lib.Sequence.sub (as_seq h1 result) 1 len in 
+    let yResult = Lib.Sequence.sub (as_seq h1 result) (1 + len) len in 
+    uint_v id == 4 /\ xResult == x /\ yResult == y))
+
 
 inline_for_extraction
-val compressionCompressedForm: #c: curve -> b: lbuffer uint8 (size 64) -> result: compressedForm -> 
+val compressionCompressedForm: #c: curve -> b: lbuffer uint8 (getCoordinateLenU c *! 2ul) -> result: compressedForm c -> 
   Stack unit 
-    (requires fun h -> live h b /\ live h result /\ disjoint b result)
-    (ensures fun h0 _ h1 -> modifies (loc result) h0 h1 /\
-      (
-        let identifier = Lib.Sequence.index (as_seq h1 result) 0 in 
-        let x = Lib.Sequence.sub (as_seq h0 b) 0 32 in 
-	  let xResult = Lib.Sequence.sub (as_seq h1 result) 1 32 in 
-        let y = Lib.Sequence.sub (as_seq h0 b) 32 32 in 
-        uint_v identifier == (Lib.ByteSequence.nat_from_intseq_be y % pow2 1)  + 2 /\
-	x == xResult	
-      )  
-  )
+  (requires fun h -> live h b /\ live h result /\ disjoint b result)
+  (ensures fun h0 _ h1 -> modifies (loc result) h0 h1 /\ (
+    let len = getCoordinateLen c in
+    
+    let identifier = Lib.Sequence.index (as_seq h1 result) 0 in 
+    let x = Lib.Sequence.sub (as_seq h0 b) 0 len in 
+    let y = Lib.Sequence.sub (as_seq h0 b) len len in 
+    let xResult = Lib.Sequence.sub (as_seq h1 result) 1 len in 
+    uint_v identifier == (Lib.ByteSequence.nat_from_intseq_be y % pow2 1) + 2 /\
+    x == xResult))
